

Definition in textbook

According to Foundations of Perturbative QCD of Collins, we have the plus function defined as below

$$\int_0^1 d\xi \left(\frac{1}{1-\xi} \right)_+ T(\xi) \equiv \int_0^1 d\xi \frac{T(\xi) - T(1)}{1-\xi} \quad (1)$$

The plus function can be effectively written as

$$\left(\frac{1}{1-\xi} \right)_+ = \frac{1}{1-\xi} - \delta(1-\xi) \int_0^1 d\xi' \frac{1}{1-\xi'} \quad (2)$$

Plus function in LaMET matching

In the LaMET matching, we have

$$f(x) = \int_0^1 dy C(x, y)_+ \tilde{f}(y) = \int_0^1 dy [C(x, y) \tilde{f}(y) - C(y, x) \tilde{f}(x)] \quad (3)$$

this can be verified by assuming $C(x, y) = \frac{1}{1-x/y} = \frac{1}{1-\xi}$, where $\xi = \frac{x}{y}$ and $dy = -x/\xi^2 d\xi$.

Using Eq. (1), the LHS of Eq. (3) becomes

$$\int_0^1 dy C(x, y)_+ \tilde{f}(y) = \int_0^1 d\xi \frac{-x}{\xi^2} \left(\frac{1}{1-\xi} \right)_+ \tilde{f}(x/\xi) = \int_0^1 d\xi \frac{1}{1-\xi} \left(\frac{-x}{\xi^2} \tilde{f}(x/\xi) - (-x \tilde{f}(x)) \right)$$

Note that the second term in the parentheses is independent on the integral variable, so we can rewrite it as

$$\int_0^1 dy C(x, y)_+ \tilde{f}(y) = \int_0^1 d\xi \frac{1}{1-\xi} \frac{-x}{\xi^2} \tilde{f}(x/\xi) + x \tilde{f}(x) \int_0^1 d\xi' \frac{1}{1-\xi'}$$

change the variable ξ back to x and y , we got

$$\begin{aligned} \int_0^1 dy C(x, y)_+ \tilde{f}(y) &= \int_0^1 dy \frac{-x}{y^2} \frac{-xy^2}{x^2} \frac{1}{1-x/y} \tilde{f}(y) + x \tilde{f}(x) \int_0^1 d\xi' \frac{1}{1-\xi'} \\ &= \int_0^1 dy \frac{\tilde{f}(y)}{1-x/y} + \tilde{f}(x) \int_0^1 d\xi' \frac{x}{1-\xi'} \end{aligned}$$

if $\xi' = y/x$, then we got

$$\int_0^1 dy C(x, y)_+ \tilde{f}(y) = \int_0^1 dy \frac{\tilde{f}(y)}{1-x/y} + \tilde{f}(x) \int_0^1 dy \frac{1}{1-y/x} = \int_0^1 dy [C(x, y) \tilde{f}(y) - C(y, x) \tilde{f}(x)]$$

The Eq. (3) is verified.

Numerical implementation of plus function

Similar to Eq. (2), we can implement the plus function in another way

$$C(x, y)_+ = C(x, y) - \delta(x-y) \int_0^1 dz C(z, y)$$

then

$$f(x) = \int_0^1 dy C(x, y)_+ \tilde{f}(y) = \int_0^1 dy C(x, y) \tilde{f}(y) - \int_0^1 dy \delta(x-y) \int_0^1 dz C(z, y) \tilde{f}(y)$$

$$= \int_0^1 dy \, C(x, y) \, \tilde{f}(y) - \int_0^1 dz \, C(z, x) \tilde{f}(x)$$

which is consistent with the definition above.

Therefore, we have

$$\begin{aligned} \int_0^1 dx \, C(x, y)_+ &= \int_0^1 dx \, C(x, y) - \int_0^1 dz \, C(z, y) = 0 \\ \int_0^1 dy \, C(x, y)_+ &= \int_0^1 dy \, C(x, y) - \int_0^1 dz \, C(z, x) \end{aligned}$$